Strengthen peg soundness result
It now states that the peg constructs parse trees that are "location
valid", and that the fringes are exact copies of the prefix of the
input that is consumed (modulo the fact that the fringe tokens are
wrapped in a TOK constructor to distinguish them from non-terminals).

compiler/parsing/proofs/pegCompleteScript.sml
@@ -863,34 +863,6 @@ val left_insert1_FOLDL = Q.store_thm(
 
 val _ = export_rewrites ["grammar.ptree_loc_def"]
 
-val merge_locs_assoc = Q.store_thm(
-  "merge_locs_assoc[simp]",
-  ‘merge_locs (merge_locs l1 l2) l3 = merge_locs l1 l3 ∧
-   merge_locs l1 (merge_locs l2 l3) = merge_locs l1 l3’,
-  map_every Cases_on [`l1`, `l2`, `l3`] >>
-  simp[locationTheory.merge_locs_def]);
-
-val merge_list_locs_2 = Q.store_thm(
-  "merge_list_locs_2[simp]",
-  ‘∀h1 h2 t.
-     merge_list_locs (h1 :: h2 :: t) = merge_list_locs (merge_locs h1 h2 :: t)’,
-  Induct_on ‘t’ >> simp[locationTheory.merge_list_locs_def]);
-
-val merge_list_locs_nested = Q.store_thm(
-  "merge_list_locs_nested[simp]",
-  ‘∀h t1 t2. merge_list_locs (merge_list_locs (h::t1) :: t2) =
-             merge_list_locs (h :: t1 ++ t2)’,
-  Induct_on ‘t1’ >> simp[locationTheory.merge_list_locs_def]);
-
-val merge_list_locs_sing = Q.store_thm(
-  "merge_list_locs_sing[simp]",
-  ‘merge_list_locs [h] = h’,
-  simp[locationTheory.merge_list_locs_def]);
-
-val merge_locs_idem = Q.store_thm(
-  "merge_locs_idem[simp]",
-  ‘merge_locs l l = l’,
-  Cases_on ‘l’ >> simp[locationTheory.merge_locs_def]);
 
 val ptree_loc_mkNd = Q.store_thm(
   "ptree_loc_mkNd[simp]",
@@ -901,58 +873,6 @@ val merge_list_locs_HDLAST = Q.store_thm(
   "merge_list_locs_HDLAST",
   ‘∀h. merge_list_locs (h::t) = merge_locs h (LAST (h::t))’,
   Induct_on ‘t’ >> simp[] >> Cases_on ‘t’ >> simp[]);
-
-val valid_locs_def = tDefine "valid_locs" ‘
-  (valid_locs (Lf _) ⇔ T) ∧
-  (valid_locs (Nd (_, l) children) ⇔
-     l = merge_list_locs (MAP ptree_loc children) ∧
-     ∀pt. MEM pt children ⇒ valid_locs pt)’
-  (WF_REL_TAC ‘measure ptree_size’ >> simp[] >> Induct >> dsimp[] >>
-   rpt strip_tac >> res_tac >> simp[]);
-val _ = export_rewrites ["valid_locs_def"]
-
-val valid_lptree_def = Define `
-  valid_lptree G pt ⇔ valid_locs pt ∧ valid_ptree G pt
-`;
-
-val valid_ptree_mkNd = Q.store_thm(
-  "valid_ptree_mkNd[simp]",
-  ‘valid_ptree G (mkNd N subs) ⇔
-     N ∈ FDOM G.rules ∧ MAP ptree_head subs ∈ G.rules ' N ∧
-     ∀pt. MEM pt subs ⇒ valid_ptree G pt’,
-  simp[mkNd_def]);
-
-val ptree_head_mkNd = Q.store_thm(
-  "ptree_head_mkNd[simp]",
-  ‘ptree_head (mkNd N subs) = NT N’,
-  simp[mkNd_def]);
-
-val ptree_list_loc_SING = Q.store_thm(
-  "ptree_list_loc_SING[simp]",
-  ‘ptree_list_loc [pt] = ptree_loc pt’,
-  simp[ptree_list_loc_def]);
-
-val ptree_fringe_mkNd = Q.store_thm(
-  "ptree_fringe_mkNd[simp]",
-  ‘ptree_fringe (mkNd N subs) = FLAT (MAP ptree_fringe subs)’,
-  simp[mkNd_def]);
-
-val valid_locs_mkNd = Q.store_thm(
-  "valid_locs_mkNd[simp]",
-  ‘valid_locs (mkNd N subs) ⇔ ∀pt. MEM pt subs ⇒ valid_locs pt’,
-  simp[mkNd_def, ptree_list_loc_def]);
-
-val valid_lptree_thm = Q.store_thm(
-  "valid_lptree_thm",
-  ‘(valid_lptree G (Lf p) ⇔ T) ∧
-   (valid_lptree G (Nd (n, l) children) ⇔
-      l = merge_list_locs (MAP ptree_loc children) ∧
-      n ∈ FDOM G.rules ∧ MAP ptree_head children ∈ G.rules ' n ∧
-      ∀pt. MEM pt children ⇒ valid_lptree G pt) ∧
-   (valid_lptree G (mkNd n children) ⇔
-      n ∈ FDOM G.rules ∧ MAP ptree_head children ∈ G.rules ' n ∧
-      ∀pt. MEM pt children ⇒ valid_lptree G pt)’,
-  simp[valid_lptree_def] >> metis_tac[]);
 
 val ptree_loc_left_insert1 = Q.store_thm(
   "ptree_loc_left_insert1",
@@ -988,13 +908,6 @@ val rightLoc_merge_locs = Q.store_thm(
 
 (* two valid parse-trees with the same head, and the same fringes, which
    are all tokens, must be identical. *)
-val real_fringe_def = tDefine "real_fringe" `
-  (real_fringe (Lf t) = [t]) ∧
-  (real_fringe (Nd n ptl) = FLAT (MAP real_fringe ptl))
-` (WF_REL_TAC `measure ptree_size` >> Induct_on `ptl` >> dsimp[] >>
-   fs[] >> rpt strip_tac >> res_tac >> simp[]);
-val _ = export_rewrites ["real_fringe_def"]
-
 
 (* Problem with Eapp is that it's left-recursive in the grammar :
 
@@ -1016,11 +929,6 @@ val _ = export_rewrites ["real_fringe_def"]
    Eapp (pt') sitting to the right, such that left-inserting the
    former into the latter gives us back what we started with.
 *)
-
-val MAP_TKI_11 = Q.store_thm(
-  "MAP_TKI_11[simp]",
-  ‘(MAP (TK ## I) l1 = MAP (TK ## I) l2) ⇔ (l1 = l2)’,
-  irule INJ_MAP_EQ_IFF >> simp[INJ_DEF, FORALL_PROD]);
 
 val eapp_reassociated = Q.store_thm(
   "eapp_reassociated",
@@ -1604,46 +1512,6 @@ in
 end g
 val normlist = REWRITE_TAC [GSYM APPEND_ASSOC, listTheory.APPEND]
 
-val SUM_MAP_FOLDR = Q.store_thm(
-  "SUM_MAP_FOLDR",
-  `SUM (MAP f l) = FOLDR (λe a. a + f e) 0 l`,
-  Induct_on `l` >> simp[]);
-
-val real_fringe_ind = theorem "real_fringe_ind"
-val LENGTH_real_fringe = Q.store_thm(
-  "LENGTH_real_fringe",
-  ‘∀pt. LENGTH (real_fringe pt) = LENGTH (ptree_fringe pt)’,
-  ho_match_mp_tac real_fringe_ind >>
-  simp[FORALL_PROD, LENGTH_FLAT, MAP_MAP_o, combinTheory.o_DEF] >>
-  simp[SUM_MAP_FOLDR] >> Induct >> simp[]);
-val rfringe_length_not_nullable = Q.prove(
-  ‘∀G s. ¬nullable G [s] ⇒
-         ∀pt. ptree_head pt = s ⇒ valid_lptree G pt ⇒
-              0 < LENGTH (real_fringe pt)’,
-  metis_tac[fringe_length_not_nullable, LENGTH_real_fringe, valid_lptree_def]);
-
-val real_fringe_mkNd = Q.store_thm(
-  "real_fringe_mkNd[simp]",
-  ‘real_fringe (mkNd n subs) = FLAT (MAP real_fringe subs)’,
-  simp[mkNd_def] >> rpt (AP_TERM_TAC ORELSE AP_THM_TAC) >>
-  simp[FUN_EQ_THM]);
-
-val ptree_head_NT_mkNd = Q.store_thm(
-  "ptree_head_NT_mkNd",
-  ‘ptree_head pt = NN n ∧ valid_lptree cmlG pt ∧
-   real_fringe pt = MAP (TK ## I) pf ⇒
-   ∃subs. pt = mkNd (mkNT n) subs’,
-  Cases_on `pt`
-  >- (rename [`ptree_head (Lf pair)`] >> Cases_on `pair` >> simp[] >>
-      rw[valid_lptree_def] >> rename [`(NN _, _) = (TK ## I) pair`] >>
-      Cases_on `pair` >> fs[]) >>
-  rename [`ptree_head (Nd pair _)`] >> Cases_on `pair` >>
-  simp[MAP_EQ_CONS, valid_lptree_thm, mkNd_def, ptree_list_loc_def]);
-
-val mkNd_11 = Q.store_thm(
-  "mkNd_11[simp]",
-  ‘mkNd n1 sub1 = mkNd n2 sub2 ⇔ n1 = n2 ∧ sub1 = sub2’,
-  csimp[mkNd_def]);
 
 val left_insert1_mkNd = Q.store_thm(
   "left_insert1_mkNd",
@@ -1729,31 +1597,35 @@ val eapp_complete = Q.store_thm(
                  REVERSE_11, listTheory.LENGTH_REVERSE] >>
   rveq >> simp[]);
 
-(*
+val leftmost_mkNd = Q.store_thm(
+  "leftmost_mkNd_DType[simp]",
+  ‘leftmost (mkNd (mkNT nDType) (c::cs)) = leftmost c’,
+  simp[leftmost_def, mkNd_def]);
+
 val leftmost_FOLDL = Q.store_thm(
   "leftmost_FOLDL",
-  `leftmost (FOLDL (λa b. Nd (mkNT nDType) [a;b]) acc args) =
+  `leftmost (FOLDL (λa b. mkNd (mkNT nDType) [a;b]) acc args) =
     leftmost acc`,
-  qid_spec_tac `acc` >> Induct_on `args` >> simp[leftmost_def]);
+  qid_spec_tac `acc` >> Induct_on `args` >> simp[]);
 
 val dtype_complete = Q.store_thm(
   "dtype_complete",
   `(∀pt' pfx' sfx' N.
-       LENGTH pfx' < LENGTH master ∧ valid_ptree cmlG pt' ∧
+       LENGTH pfx' < LENGTH master ∧ valid_lptree cmlG pt' ∧
        mkNT N ∈ FDOM cmlPEG.rules ∧
-       ptree_head pt' = NN N ∧ ptree_fringe pt' = MAP TK pfx' ∧
-       (sfx' ≠ [] ⇒ HD sfx' ∈ stoppers N) ⇒
+       ptree_head pt' = NN N ∧ real_fringe pt' = MAP (TK ## I) pfx' ∧
+       (sfx' ≠ [] ⇒ FST (HD sfx') ∈ stoppers N) ⇒
        peg_eval cmlPEG (pfx' ++ sfx', nt (mkNT N) I) (SOME(sfx', [pt']))) ∧
     (∀pt' sfx'.
-       valid_ptree cmlG pt' ∧ ptree_head pt' = NN nTbase ∧
-       ptree_fringe pt' = MAP TK master ∧
-       (sfx' ≠ [] ⇒ HD sfx' ∈ stoppers nEbase) ⇒
+       valid_lptree cmlG pt' ∧ ptree_head pt' = NN nTbase ∧
+       real_fringe pt' = MAP (TK ## I) master ∧
+       (sfx' ≠ [] ⇒ FST (HD sfx') ∈ stoppers nEbase) ⇒
        peg_eval cmlPEG (master ++ sfx',nt (mkNT nTbase) I) (SOME (sfx', [pt'])))
     ⇒
      ∀pfx apt sfx.
-       IS_SUFFIX master pfx ∧ valid_ptree cmlG apt ∧
-       ptree_head apt = NN nDType ∧ ptree_fringe apt = MAP TK pfx ∧
-       (sfx ≠ [] ⇒ HD sfx ∈ stoppers nDType) ⇒
+       IS_SUFFIX master pfx ∧ valid_lptree cmlG apt ∧
+       ptree_head apt = NN nDType ∧ real_fringe apt = MAP (TK ## I) pfx ∧
+       (sfx ≠ [] ⇒ FST (HD sfx) ∈ stoppers nDType) ⇒
        peg_eval cmlPEG (pfx ++ sfx, nt (mkNT nDType) I) (SOME(sfx, [apt]))`,
   strip_tac >>
   simp[Once peg_eval_NT_SOME, cmlpeg_rules_applied, (*list_case_lemma, *)
@@ -1762,14 +1634,15 @@ val dtype_complete = Q.store_thm(
   completeInduct_on `LENGTH pfx` >> qx_gen_tac `pfx` >> strip_tac >>
   rveq >> fs[GSYM RIGHT_FORALL_IMP_THM] >>
   map_every qx_gen_tac [`apt`, `sfx`] >> strip_tac >>
-  `∃subs. apt = Nd (mkNT nDType) subs`
-    by (Cases_on `apt` >> fs[MAP_EQ_CONS] >> rw[]) >>
-  fs[MAP_EQ_CONS, MAP_EQ_APPEND, cmlG_FDOM, cmlG_applied] >> rw[] >>
+  `∃subs. apt = mkNd (mkNT nDType) subs`
+    by metis_tac[ptree_head_NT_mkNd] >>
+  fs[MAP_EQ_CONS, MAP_EQ_APPEND, cmlG_FDOM, cmlG_applied, valid_lptree_thm] >>
+  rw[] >>
   fs[MAP_EQ_CONS, MAP_EQ_APPEND, DISJ_IMP_THM, FORALL_AND_THM] >> rw[]
-  >- (asm_match `ptree_head apt = NN nDType` >>
-      asm_match `ptree_fringe apt = MAP TK af` >>
-      asm_match `ptree_head bpt = NN nTyOp` >>
-      asm_match `ptree_fringe bpt = MAP TK bf` >>
+  >- (rename [`ptree_head apt = NN nDType`,
+              `real_fringe apt = MAP _ af`,
+              `ptree_head bpt = NN nTyOp`,
+              `real_fringe bpt = MAP _ bf`] >>
       qspecl_then [`apt`, `bpt`, `af`, `bf`] mp_tac dtype_reassociated >>
       simp[MAP_EQ_APPEND, GSYM LEFT_EXISTS_AND_THM, GSYM RIGHT_EXISTS_AND_THM]>>
       disch_then (qxchl [`apt'`, `bpt'`, `bf'`, `af'`] strip_assume_tac) >>
@@ -1779,8 +1652,8 @@ val dtype_complete = Q.store_thm(
         by (Q.UNDISCH_THEN `af ++ bf = bf' ++ af'` SUBST_ALL_TAC >>
             fs[rich_listTheory.IS_SUFFIX_compute] >>
             imp_res_tac rich_listTheory.IS_PREFIX_LENGTH >> fs[]) >>
-      erule mp_tac (MATCH_MP fringe_length_not_nullable nullable_Tbase) >>
-      erule mp_tac (MATCH_MP fringe_length_not_nullable nullable_DType) >>
+      erule mp_tac (MATCH_MP rfringe_length_not_nullable nullable_Tbase) >>
+      erule mp_tac (MATCH_MP rfringe_length_not_nullable nullable_DType) >>
       simp[] >> ntac 2 strip_tac >>
       `LENGTH (bf' ++ af') ≤ LENGTH master` by metis_tac[] >> fs[] >>
       conj_tac
